Makefile
@@ -195,7 +195,7 @@ CLOSE=SmallstepClosed.v CompilerClosed.v
 CONCUR=MultiLibs.v CMulti.v AsmMulti.v \
        CallconvBig.v MultiSimBig.v \
        HCompBig.v InjpAccoComp.v VCompBig.v \
-       SimplLocalsproofC.v CminorgenproofC.v \
+       SimplLocalsproofC.v CminorgenproofC.v InliningproofC.v \
        Composition.v
 
 
